<?xml version="1.0" encoding="UTF-8"?>

<section xml:id="s_lim_rules" xmlns:xi="http://www.w3.org/2001/XInclude">
    <title>Limit rules</title>
    <objectives>
        <ol>
            <li>
                <p>
                    State and apply limit rules to compute limits of functions formed from other functions using arithmetic operations.
                </p>
            </li>
            <li>
                <p>
                    Understand that a limit rule can only be applied subjecto to certain restrictions. 
                </p>
            </li>
            <li>
                <p>
                    See examples where limit rules are not sufficient for computing a limit. 
                </p>
            </li>
        </ol>
    </objectives>
    <subsection xml:id="ss_limit_laws">
        <title>Limit rules</title>
    <p>
        We now state some useful limit formulas and rules. These will give us a means of breaking down the limit computation of a complicated function into limits of simpler functions. Technically speaking we must prove the validity of each of these rules and formulas; however this would be a fool's errand until we have a rigorous definition of the limit to work with! Such a definition will be provided in the near future, though even then we will not concern ourselves overly with proofs; we are more interested in learning how to make valid use of the rules. 
    </p>
    <p>
        Our first theorem gives us two simple <em>formulas</em> for computing the limits of particular types of functions: constant functions, and the identity function. 
    </p>
    <theorem xml:id="th_lim_const_id">
    <title>Constant and identity functions</title>
        <statement>
            <p>
            <ol>  
                <li xml:id="th_lim_const">
                    <title>Constant function</title>
                    <p>
                       Fix a real number <m>c\in \R</m> and let <m>h\colon \R\rightarrow \R</m> be the constant function defined as <m>h(x)=c</m> for all <m>x\in \R</m>. Given any <m>a\in \R</m> we have 
                       <men xml:id="eq_limit_const">
                        \lim_{x\to a}h(x)=\lim_{x\to a}c=c
                       </men>.
                    </p>
                </li>
                <li xml:id="th_lim_id">
                    <title>Identity function</title>
                    <p>
                       Let <m>\id\colon \R\rightarrow \R</m> be the identity function defined as <m>\id(x)=x</m> for all <m>x\in \R</m>. Given any <m>a\in \R</m> we have 
                       <men xml:id="eq_lim_id">
                        \lim_{x\to a}\id(x)=\lim_{x\to a}x=a
                       </men>.
                    </p>
                </li>
            </ol> 
            </p>
        </statement>
    </theorem>
    <p>
        In contrast to the last theorem, our next theorem does not provide any formulas per se, but rather gives us <em>rules</em> governing how limits interact with various function operations like addition, multiplication, <etc/>. 
    </p>
    <theorem xml:id="th_lim_rules">
        <title>Limit rules</title>
        <statement>
            <p>
               Let <m>f</m> and <m>g</m> be functions, and suppose <m>\lim\limits_{x\to a}f(x)</m> and <m>\lim\limits_{x\to a}g(x)</m> exist for the real number <m>a\in \R</m>. 
            <ol>
                <li xml:id="th_lim_sum">
                    <title>Sum rule</title>
                    <p>
                       <m>\lim\limits_{x\to a}
                        \left(f(x)+g(x)\right)=\lim\limits_{x\to a}f(x)+\lim\limits_{x\to a}g(x)</m>.
                    </p>
                </li>
                <li xml:id="th_lim_diff">
                    <title>Difference rule</title>
                    <p>
                        <m>\lim\limits_{x\to a}\left(f(x)-g(x)\right)=\lim\limits_{x\to a}f(x)-\lim\limits_{x\to a}g(x)</m>.
                    </p>
                </li>
                <li xml:id="th_scal_mult">
                    <title>Scalar multiple rule</title>
                    <p>
                        <m>\lim\limits_{x\to a}\left(cf(x)\right)=c\lim\limits_{x\to a}f(x)</m> for all <m>c\in \R</m>. 
                    </p>
                </li>
                <li xml:id="th_prod">
                    <title>Product rule</title>
                    <p>
                        <m>\lim\limits_{x\to a}\left(f(x)g(x)\right)=\lim\limits_{x\to a}f(x)\, \lim\limits_{x\to a}g(x)</m>.
                    </p>
                </li>
                <li xml:id="th_lim_quot">
                    <title>Quotient rule</title>
                    <p>
                       If <m>\lim\limits_{x\to a}g(x)\ne 0</m>, then 
                       <m>\displaystyle
                        \lim\limits_{x\to a}\frac{f(x)}{g(x)}=\frac{\lim\limits_{x\to a}f(x)}{\lim\limits_{x\to a}g(x)}
                       </m>.
                    </p>
                </li>
                <li xml:base="th_lim_power">
                    <title>Power rule</title>
                    <p>
                        <m>\lim\limits_{x\to a}[f(x)]^n=\left[\lim\limits_{x\to a}f(x)\right]^n</m> for all positive integers <m>n</m>. 
                    </p>
                </li>
                <li xml:base="th_lim_root">
                    <title>Root rule</title>
                    <p>
                        <m>\lim\limits_{x\to a}\sqrt[n]{f(x)}=\sqrt[n]{\lim\limits_{x\to a}f(x)}</m> for all positive integers <m>n</m>, where we must assume <m>\lim\limits_{x\to a}f(x)</m> is positive if <m>n</m> is even. 
                    </p>
                </li>
                <li xml:id="th_lim_repl">
                    <title>Replacement rule</title>
                    <p>
                        If <m>h</m> is a function satisfying <m>h(x)=f(x)</m> for all <m>x\ne a</m> in an open interval about <m>a</m>, then <m>\lim\limits_{x\to a}f(x)=\lim\limits_{x\to a}h(x)</m>.
                    </p>
                </li>
            </ol>
            </p>

        </statement>
    </theorem>
    <remark>
        <title>Limit rules</title>
        <p>
            It is useful to think of <xref ref="th_lim_rules"/> as giving us a bunch of algebraic rules for computing limits of functions defined using addition, subtraction, multiplication, etc. For the most part these rules tell us that we can <q>bring the limit into</q> various operations: for example, the first two rules tell us that we can bring the limit into sums and differences of functions.
            Or better, using plain English, they tell us that the limit of a sum (of functions) is the sum of the limits, and that the limit of a difference (of functions) is the difference of the limits.
        </p>
        <p>
            In fact most of the rules in <xref ref="th_lim_rules"/> can be nicely summarized in plain English (<eg/>, <q>the limit of a product is the product of the limits</q>, <q>the limit of an <m>n</m>-th power is the <m>n</m>-th power of the limit </q>), and these summaries are helpful for remembering how the limit interacts with function operations.
        </p>
    </remark>
    <remark>
        <title>Quotient rule</title>
        <p>
            Assume as in <xref ref="th_lim_rules"/> that <m>\lim_{x\to a}f(x)</m> and <m>\lim_{x\to a}g(x)</m> exist and consider the limit <m>\lim_{x\to a}\frac{f(x)}{g(x)}</m>. Mark well that we can only make use of the quotient rule if <m>\lim_{x\to a}g(x)\ne 0</m>, in which case we can conclude that the limit of the quotient is the quotient of the limits. 
        </p>
        <p>
            Note further that in the case where <m>\lim_{x\to a}g(x)=0</m>, we cannot automatically conclude that the limit <m>\lim_{x\to a}\frac{f(x)}{g(x)}</m> does not exist; it simply the case that we cannot make use of the quotient rule to evaluate this limit. When this happens, we must look to other means for investigating the limit. See <xref ref="eg_lim_quot_fail"/>.
        </p>
    </remark>
    <example xml:id="eg_lim_rules">
    <title>Using limit rules</title>
    <statement>
    <p>
    Compute the following limits. 
    <ol>
        <li>
            <p>
                <m>\lim\limits_{t\to 6}8(t-5)(t-7)</m>
            </p>
        </li>
        <li>
            <p>
                <m>\lim\limits_{x\to -2}x^3-4x+8</m>
            </p>
        </li>
        <li>
            <p>
                <m>\lim\limits_{z\to 4}\sqrt{z^2-10}</m>
            </p>
        </li>
        <li>
            <p>
                <m>\lim\limits_{y\to 2}\frac{y+2}{y^2+5y+6}</m>
            </p>
        </li>
    </ol>
    </p>
    </statement>
    <solution>
    <p>
    
    </p>
    </solution>
    </example>
    
    <example xml:id="eg_lim_rule_complic">
        <title>Using limit rules</title>
        <statement><p>
            Compute the limit below. Your answer should be a <em>chain of equalities</em> with steps justified by limit rules. 
            <me>
                \lim_{x\to -2}\frac{x^3+x+1}{\sqrt[3]{4x^2+11}}
            </me>
            
        </p></statement>
        <solution>
            <p>
                <md>
                    <mrow>\lim_{x\to -2}\frac{x^3+x+1}{\sqrt[3]{4x^2+11}} \amp = \frac{\lim\limits_{x\to -2}(x^3+x+1)}{\lim\limits_{x\to -2}\sqrt[3]{4x^2+11}}
                        \amp \text{(quot. rule)}
                    </mrow>
                    <mrow> \amp =\frac{(\lim\limits_{x\to -2}x)^3+\lim\limits_{x\to -2}x+\lim\limits_{x\to -2}1}{\sqrt[3]{\lim\limits_{x\to -2}(4x^2+11)}}
                        \amp \text{(sum, power rule/root rule)}
                    </mrow>
                    <mrow> \amp =\frac{(-2)^3-2+1}{\sqrt[3]{\lim_{x\to -2}(4x^2)+\lim\limits_{x\to -2}11}}
                        \amp \text{(ident., const. rule/sum rule)}
                    </mrow>
                    <mrow> \amp =\frac{-9}{\sqrt[3]{4(\lim\limits_{x\to -2}x)^2+11}}
                        \amp \text{(scal. mult., power, const. rule)}
                    </mrow>
                    <mrow> \amp =-\frac{9}{\sqrt[3]{4(-2)^2+11}} \amp \text{(ident. rule)}</mrow>
                    <mrow> \amp =-\frac{9}{\sqrt[3]{27}}=-3</mrow>
                </md>.
            </p>
        </solution>
    </example>
    <corollary xml:id="cor_poly_rational">
        <title>Evaluation (polynomials and rational functions)</title>
        <statement>
            <p>
                <ol>
                    <li>
                        <title>Polynomial evaluation</title>
                        <p>
                            Let <m>f(x)=\anpoly</m> be a polynomial. Given any <m>a\in \R</m>, we have 
                            <me>
                                \lim\limits_{x\to a}f(x)=f(a)
                            </me>.
                        </p>
                    </li>
                    <li>
                        <title>Rational evaluation</title>
                        <p>
                            Let <m>f</m> and <m>g</m> be polynomials. For any <m>a\in \R</m> satisfying <m>g(a)\ne 0</m>, we have 
                            <me>
                                \lim\limits_{x\to a}\frac{f(x)}{g(x)}=\frac{f(a)}{g(a)}
                            </me>.
                        </p>
                    </li>
                </ol>
            </p>
        </statement>
    </corollary>
    <example xml:id="eg_poly_eval">
        <title>Polynomial evaluation</title>
        <statement><p>
            Give a simplified computation of the limit in <xref ref="eg_lim_rules_complic"/> using <xref ref="cor_poly_rational"/>.
        </p></statement>
        <solution>
            <p>
                The polynomial evaluation formula allows us to skip a few steps in our computation from <xref ref="eg_lim_rules"/>:
                <md>
                    <mrow>\lim_{x\to -2}\frac{x^3+x+1}{\sqrt[3]{4x^2+11}} \amp = \frac{\lim\limits_{x\to -2}(x^3+x+1)}{\lim\limits_{x\to -2}\sqrt[3]{4x^2+11}}
                        \amp \text{(quot. rule)}
                    </mrow>
                    <mrow> \amp =\frac{(-2)^3+(-2)+1}{\sqrt[3]{\lim\limits_{x\to -2}(4x^2+11)}}
                        \amp \text{(poly. eval./root rule)}
                    </mrow>
                    <mrow> \amp =\frac{-9}{\sqrt[3]{4(-2)^2+11}}
                        \amp \text{(poly eval.)}
                    </mrow>
                    <mrow> \amp =-\frac{9}{\sqrt[3]{27}}=-3</mrow>
                </md>.
            </p>
        </solution>
    </example>
    <example xml:id="eg_lim_quot_fail">
        <title>Quotient rule does not apply</title>
        <statement><p>
            Compute the limit below. Your answer should be a chain of equalities with each step justified. 
            <me>
                \lim_{x\to 1}\frac{x^2-1}{x-1}
            </me>
            
        </p></statement>
        <solution>
            <p>
                Note that since the limit of the denominator function is 0, we are not able to use the quotient (or rational function) rule. We begin instead with some algebra: 
                <md>
                    <mrow> \lim_{x\to 1}\frac{x^2-1}{x-1}\amp =\lim_{x\to 1}\frac{(x-1)(x+1)}{x-1} </mrow>
                    <mrow> \amp = \lim_{x\to 1}x+1 \amp \text{(repl. rule)}</mrow>
                    <mrow> \amp =2 \amp \text{(poly eval.)}</mrow>
                </md>. 
            </p>
        </solution>
    </example>
    </subsection>
    

</section>